More progress on fp2imp + fix some derivations

coq/theories/assembly/ASMToString.v
@@ -8,7 +8,8 @@ From impboot Require Import commons.PrintingUtils.
 
 Open Scope string.
 
-Definition reg2str (r: reg) (str: string): string :=
+(* This is named reg2str1, since when I named it reg2str, it reified forever, see example in AsmToStringDerivations.v *)
+Definition reg2str1 (r: reg) (str: string): string :=
   match r with
   | RAX => "%rax"
   | RDI => "%rdi"
@@ -40,31 +41,31 @@ Fixpoint clean (cs: string) (acc: string): string :=
 
 Definition inst2str (i: instr) (str: string): string :=
   match i with
-  | Const r imm => "movq $" ++ N2str (Z.to_N (word.unsigned imm)) (", " ++ reg2str r str)
-  | Mov dst src => "movq " ++ reg2str src (", " ++ reg2str dst str)
-  | ASMSyntax.Add dst src => "addq " ++ reg2str src (", " ++ reg2str dst str)
-  | Sub dst src => "subq " ++ reg2str src (", " ++ reg2str dst str)
-  | Div r => "divq " ++ reg2str r str
+  | Const r imm => "movq $" ++ N2str (Z.to_N (word.unsigned imm)) (", " ++ reg2str1 r str)
+  | Mov dst src => "movq " ++ reg2str1 src (", " ++ reg2str1 dst str)
+  | ASMSyntax.Add dst src => "addq " ++ reg2str1 src (", " ++ reg2str1 dst str)
+  | Sub dst src => "subq " ++ reg2str1 src (", " ++ reg2str1 dst str)
+  | Div r => "divq " ++ reg2str1 r str
   | Jump cond n =>
     match cond with
     | Always => "jmp " ++ lab n str
     | Equal r1 r2 =>
-      "cmpq " ++ reg2str r2 (", " ++ reg2str r1 (" ; je " ++ lab n str))
+      "cmpq " ++ reg2str1 r2 (", " ++ reg2str1 r1 (" ; je " ++ lab n str))
     | Less r1 r2 =>
-      "cmpq " ++ reg2str r2 (", " ++ reg2str r1 (" ; jb " ++ lab n str))
+      "cmpq " ++ reg2str1 r2 (", " ++ reg2str1 r1 (" ; jb " ++ lab n str))
     end
   | Call n => "call " ++ lab n str
   | Ret => "ret" ++ str
-  | Pop r => "popq " ++ reg2str r str
-  | Push r => "pushq " ++ reg2str r str
-  | Load_RSP r n => "movq " ++ num2str (8 * n) ("(%rsp), " ++ reg2str r str)
-  | Store_RSP r n => "movq " ++ (reg2str r (", " ++ num2str (8 * n) ("(%rsp), " ++ str)))
+  | Pop r => "popq " ++ reg2str1 r str
+  | Push r => "pushq " ++ reg2str1 r str
+  | Load_RSP r n => "movq " ++ num2str (8 * n) ("(%rsp), " ++ reg2str1 r str)
+  | Store_RSP r n => "movq " ++ (reg2str1 r (", " ++ num2str (8 * n) ("(%rsp), " ++ str)))
   | Add_RSP n => "addq $" ++ num2str (8 * n) (", %rsp" ++ str)
   | Sub_RSP n => "subq $" ++ num2str (8 * n) (", %rsp" ++ str)
   | Store src a w =>
-      "movq " ++ reg2str src (", " ++ N2str (Z.to_N (word.unsigned w)) ("(" ++ reg2str a (")" ++ str)))
+      "movq " ++ reg2str1 src (", " ++ N2str (Z.to_N (word.unsigned w)) ("(" ++ reg2str1 a (")" ++ str)))
   | Load dst a w =>
-      "movq " ++ N2str (Z.to_N (word.unsigned w)) ("(" ++ reg2str a ("), " ++ reg2str dst str))
+      "movq " ++ N2str (Z.to_N (word.unsigned w)) ("(" ++ reg2str1 a ("), " ++ reg2str1 dst str))
   | GetChar => "movq stdin(%rip), %rdi ; call _IO_getc@PLT" ++ str
   | PutChar => "movq stdout(%rip), %rsi ; call _IO_putc@PLT" ++ str
   | Exit => "call exit@PLT" ++ str
